Add Clause.shrink

BSWLean/Substitutions.lean
@@ -7,10 +7,36 @@ def Literal.restrict {vars} (l : Literal vars)
   | .pos v _ => Literal.pos v h_mem
   | .neg v _ => Literal.neg v h_mem
 
+lemma Literal.restrict_inj {vars} (l₁ : Literal vars) (l₂ : Literal vars)
+  (sub_vars : Variables) (h_l₁_mem : l₁.variable ∈ sub_vars) (h_l₂_mem : l₂.variable ∈ sub_vars)
+  : l₁.restrict sub_vars h_l₁_mem = l₂.restrict sub_vars h_l₂_mem → l₁ = l₂ := by
+  intros h_eq
+  unfold Literal.restrict at h_eq
+  cases l₁ <;> cases l₂ <;> simp_all
+
 def Clause.shrink {vars} (c : Clause vars)
     (keep_vars : Variables) (h_mem : ∀ l, l ∈ c → l.variable ∈ keep_vars)
     : Clause keep_vars :=
-  sorry
+  let f := fun l : Literal vars =>
+      if h : l ∈ c then some (l.restrict keep_vars (h_mem l h)) else none
+
+  have : ∀ l₁ l₂, ∀ r ∈ f l₁, r ∈ f l₂ → l₁ = l₂ := by
+    intros l₁ l₂ b h₁ h₂
+    unfold f at h₁ h₂
+    simp_all only [Option.mem_def, Option.dite_none_right_eq_some, Option.some.injEq]
+    obtain ⟨_, h⟩ := h₁
+    obtain ⟨h_l₂_c, h_l₂_b⟩ := h₂
+    rw [←h_l₂_b] at h
+    have h_l₁_vars : l₁.variable ∈ keep_vars := by (expose_names; exact h_mem l₁ w)
+    have h_l₂_vars : l₂.variable ∈ keep_vars := by (expose_names; exact h_mem l₂ h_l₂_c)
+    unfold Literal.restrict at h
+    expose_names;
+    exact
+      Literal.restrict_inj l₁ l₂ keep_vars
+        (h_mem l₁ ((Iff.of_eq (Eq.refl (l₁ ∈ c))).mpr w))
+        (h_mem l₂ ((Iff.of_eq (Eq.refl (l₂ ∈ c))).mpr h_l₂_c)) h
+
+  c.filterMap f this
 
 def Clause.split {vars} (c : Clause vars)
     (split_vars : Variables)
@@ -49,6 +75,12 @@ def Assignment.restrict {vars} (ρ : Assignment vars)
 
   fun v h_v_mem_sub_vars => ρ v (this v h_v_mem_sub_vars)
 
+lemma Literal.restrict_correctness {vars} (l : Literal vars) (sub_vars : Variables)
+  (ρ : Assignment vars) (h_subset : sub_vars ⊆ vars) (h_l : l.variable ∈ sub_vars)
+  : l.eval ρ = (l.restrict sub_vars h_l).eval (ρ.restrict sub_vars h_subset) := by
+  sorry
+
+
 def Clause.substitute {vars} (c : Clause vars)
     (sub_vars : Variables) (ρ : Assignment sub_vars)
     : Option (Clause (vars \ sub_vars)) :=
@@ -78,9 +110,79 @@ lemma Assignment.restrict_correctness {vars} {h} (ρ : Assignment vars)
 
 lemma Clause.split_correctness {vars} (c : Clause vars)
     (sub_vars : Variables) (ρ : Assignment vars) (h₁) (h₂) :
-    c.eval ρ = (c.split sub_vars).1.eval (ρ.restrict (vars ∩ sub_vars) h₁)
-            || (c.split sub_vars).2.eval (ρ.restrict (vars \ sub_vars) h₂) := by
-  sorry
+    c.eval ρ = ((c.split sub_vars).1.eval (ρ.restrict (vars ∩ sub_vars) h₁)
+            || (c.split sub_vars).2.eval (ρ.restrict (vars \ sub_vars) h₂)) := by
+  by_cases h_c : c.eval ρ
+
+  case pos =>
+    rw [h_c]
+    simp only [Bool.true_eq, Bool.or_eq_true]
+    rw [Clause.eval_eq_true_iff_exists_satisfied_literal] at h_c
+    obtain ⟨l, h_l_in_c, h_l_eval_ρ⟩ := h_c
+    by_cases h_l_in_c_in : l.variable ∈ sub_vars
+    case pos =>
+      left
+      rw [Clause.eval_eq_true_iff_exists_satisfied_literal]
+      let l' := l.restrict (vars ∩ sub_vars) (by
+        simp only [Finset.mem_inter, Literal.variable_mem_vars, true_and]
+        exact h_l_in_c_in
+      )
+      have h_unfold : l' = l.restrict (vars ∩ sub_vars) (by
+        simp only [Finset.mem_inter, Literal.variable_mem_vars, true_and]
+        exact h_l_in_c_in
+      ) := by
+        sorry
+      have h_l'_in_c_in : l' ∈ (c.split sub_vars).1 := by
+        unfold Clause.split
+        simp only
+        unfold Clause.shrink
+        simp only [Finset.mem_filter, Finset.mem_filterMap, Option.dite_none_right_eq_some,
+          Option.some.injEq, and_exists_self]
+        use l
+        have : l ∈ c ∧ l.variable ∈ sub_vars := by
+          constructor
+          · assumption
+          · assumption
+        use this
+      have h_l'_eval : l'.eval (ρ.restrict (vars ∩ sub_vars) h₁) := by
+        rw [h_unfold]
+        rw [←Literal.restrict_correctness l (vars ∩ sub_vars) ρ]
+        assumption
+
+      use l'
+    case neg =>
+      right
+      rw [Clause.eval_eq_true_iff_exists_satisfied_literal]
+      let l' := l.restrict (vars \ sub_vars) (by
+        simp only [Finset.mem_sdiff, Literal.variable_mem_vars, true_and]
+        exact h_l_in_c_in
+      )
+      have h_unfold : l' = l.restrict (vars \ sub_vars) (by
+        simp only [Finset.mem_sdiff, Literal.variable_mem_vars, true_and]
+        exact h_l_in_c_in
+      ) := by
+        sorry
+      have h_l'_in_c_in : l' ∈ (c.split sub_vars).2 := by
+        unfold Clause.split
+        simp only
+        unfold Clause.shrink
+        simp only [Finset.mem_filter, Finset.mem_filterMap, Option.dite_none_right_eq_some,
+          Option.some.injEq, and_exists_self]
+        use l
+        have : l ∈ c ∧ l.variable ∉ sub_vars := by
+          constructor
+          · assumption
+          · assumption
+        use this
+      have h_l'_eval : l'.eval (ρ.restrict (vars \ sub_vars) h₂) := by
+        rw [h_unfold]
+        rw [←Literal.restrict_correctness l (vars \ sub_vars) ρ]
+        assumption
+
+      use l'
+
+  case neg =>
+    sorry
 
 
 def CNFFormula.substitute {vars} (φ : CNFFormula vars)
