BSWLean.lean
@@ -1,2 +1,3 @@
 import BSWLean.CNF
 import BSWLean.Treelike
+import BSWLean.Substitutions
